Plfl/IMP.lean
@@ -1,0 +1,115 @@
+def Loc := String deriving Repr, BEq
+
+inductive Aexp : Type :=
+  | num : Nat → Aexp
+  | var : Loc → Aexp
+  | add : Aexp → Aexp → Aexp
+  | sub : Aexp → Aexp → Aexp
+  | mul : Aexp → Aexp → Aexp
+  deriving Repr
+
+prefix:90 "% " => Aexp.num
+prefix:90 "` " => Aexp.var
+infixl:65 " +ᵃ " => Aexp.add
+infixl:65 " -ᵃ " => Aexp.sub
+infixl:70 " *ᵃ " => Aexp.mul
+
+#eval %1 +ᵃ %2
+
+inductive Bexp : Type
+  | tru : Bexp
+  | fls : Bexp
+  | eq  : Aexp → Aexp → Bexp
+  | le  : Aexp → Aexp → Bexp
+  | not : Bexp → Bexp
+  | and : Bexp → Bexp → Bexp
+  | or  : Bexp → Bexp → Bexp
+
+notation "true" => Bexp.tru
+notation "false" => Bexp.fls
+infix:50 " =ᵇ " => Bexp.eq
+infix:50 " ≤ᵇ " => Bexp.le
+prefix:85 "¬ᵇ " => Bexp.not
+infixr:35 " ∧ᵇ " => Bexp.and
+infixr:30 " ∨ᵇ " => Bexp.or
+
+inductive Com : Type
+  | skip  : Com
+  | asg   : Loc → Aexp → Com
+  | seq   : Com → Com → Com
+  | ite   : Bexp → Com → Com → Com
+  | while : Bexp → Com → Com
+
+notation "skip" => Com.skip
+infix:60 " ≔ " => Com.asg
+infix:65 " ; " => Com.seq
+notation:60 "if" b "then" c₁:60 "else" c₂:60 => Com.ite b c₁ c₂
+notation:60 "while" b "do_" c => Com.while b c
+
+def State := Loc → Nat
+
+inductive AEval : Aexp → State → Nat → Prop
+  | num {n σ} : AEval (% n) σ n
+  | var {x σ} : AEval (` x) σ (σ x)
+  | add {a₀ a₁ n₀ n₁ σ} :
+      AEval a₀ σ n₀ →
+      AEval a₁ σ n₁ →
+      AEval (a₀ +ᵃ a₁) σ (n₀ + n₁)
+  | sub {a₀ a₁ n₀ n₁ σ} :
+      AEval a₀ σ n₀ →
+      AEval a₁ σ n₁ →
+      AEval (a₀ -ᵃ a₁) σ (n₀ - n₁)
+  | mul {a₀ a₁ n₀ n₁ σ} :
+      AEval a₀ σ n₀ →
+      AEval a₁ σ n₁ →
+      AEval (a₀ *ᵃ a₁) σ (n₀ * n₁)
+
+inductive BEval : Bexp → State → Bool → Prop
+  | tru {σ} : BEval true σ Bool.true
+  | fls {σ} : BEval false σ Bool.false
+  | eq {a₀ a₁ n₀ n₁ σ} :
+      AEval a₀ σ n₀ →
+      AEval a₁ σ n₁ →
+      BEval (a₀ =ᵇ a₁) σ (n₀ == n₁)
+  | le {a₀ a₁ n₀ n₁ σ} :
+      AEval a₀ σ n₀ →
+      AEval a₁ σ n₁ →
+      BEval (a₀ ≤ᵇ a₁) σ (n₀ <= n₁)
+  | not {b b' σ} :
+      BEval b σ b' →
+      BEval (¬ᵇ b) σ (!b')
+  | and {b₀ b₁ t₀ t₁ σ} :
+      BEval b₀ σ t₀ →
+      BEval b₁ σ t₁ →
+      BEval (b₀ ∧ᵇ b₁) σ (t₀ && t₁)
+  | or {b₀ b₁ t₀ t₁ σ} :
+      BEval b₀ σ t₀ →
+      BEval b₁ σ t₁ →
+      BEval (b₀ ∨ᵇ b₁) σ (t₀ || t₁)
+
+def ext (σ : State) (m : Nat) (x : Loc) : State :=
+  fun y => if y == x then m else σ y
+
+notation:70 σ "[" m "⧸" x "]" => ext σ m x
+
+inductive CEval : Cexp → State → State → Prop
+  | skip {σ} : CEval skip σ σ
+  | ass {a σ m x} : AEval a σ m → CEval (x ≔ a) σ (σ [m ⧸ x])
+  | seq {c₀ c₁ σ σ' σ''} :
+      CEval c₀ σ σ'' →
+      CEval c₁ σ'' σ' →
+      CEval (c₀ ; c₁) σ σ'
+  | itetru {b σ c₀ σ'} :
+      BEval b σ Bool.true →
+      CEval c₀ σ σ' →
+      CEval (if b then c₀ else c₁) σ σ'
+  | itefls {b σ c₀ σ'} :
+      BEval b σ Bool.true →
+      CEval c₁ σ σ' →
+      CEval (if b then c₀ else c₁) σ σ'
+  | whilefls {b σ c} :
+      BEval b σ Bool.false →
+      CEval (while b do_ c) σ σ
+  | whiletru {b σ c} :
+      BEval b σ Bool.false →
+      CEval (while b do_ c) σ σ
